ci + bw-comp

theories/gitree/reify.v
@@ -25,6 +25,13 @@ Section reifiers.
   Implicit Type op : opid F.
   Implicit Type α β : IT.
 
+  Class CtxIndep (X : ofe) `{!Cofe X} (op : opid F) := {
+      cont_irrelev :
+      (∃ f : (prodO (Ins (sReifier_ops r _) ♯ X) ((sReifier_state r) ♯ X)) -n>
+               optionO (prodO (Outs (sReifier_ops r _) ♯ X) (sReifier_state r ♯ X)),
+         ∀ i σ κ, @sReifier_re _ X _ op (i, σ, κ) ≡ fmap (prodO_map κ idfun) (f (i, σ)));
+    }.
+
   Notation stateM := ((stateF ♯ IT -n> (stateF ♯ IT) * IT)).
   #[local] Instance stateT_inhab : Inhabited stateM.
   Proof.
@@ -239,95 +246,95 @@ Section reifiers.
       reflexivity.
   Qed.
 
-  (* Lemma reify_vis_cont op i k1 (k2 : IT -n> IT) σ1 σ2 β *)
-  (*   {PROP : bi} `{!BiInternalEq PROP} (H : IT_hom k2) : *)
-  (*   (reify (Vis op i k1) σ1 ≡ (σ2, Tick β) ⊢ *)
-  (*    reify (Vis op i (laterO_map k2 ◎ k1)) σ1 ≡ (σ2, Tick (k2 β)) : PROP)%I. *)
-  (* Proof. *)
-  (*   destruct (sReifier_re r op (i, σ1, k1)) as [[o σ2']|] eqn:Hre; last first. *)
-  (*   - rewrite (reify_vis_None _ _ k1); last by rewrite Hre//. *)
-  (*     iIntros "Hr". iExFalso. *)
-  (*     iPoseProof (prod_equivI with "Hr") as "[_ Hk]". *)
-  (*     simpl. iApply (IT_tick_err_ne). by iApply internal_eq_sym. *)
-  (*   - rewrite reify_vis_eq; last first. *)
-  (*     { by rewrite Hre. } *)
-  (*     iIntros "Hr". *)
-  (*     iPoseProof (prod_equivI with "Hr") as "[Hs Hk]". *)
-  (*     iPoseProof (Tau_inj' with "Hk") as "Hk". *)
-  (*     iAssert (reify (Vis op i (laterO_map k2 ◎ k1)) σ1 ≡ (reify (k2 (Vis op i k1)) σ1))%I as "HEQ". *)
-  (*     { *)
-  (*       iPureIntro. *)
-  (*       do 2 f_equiv. *)
-  (*       rewrite hom_vis. *)
-  (*       f_equiv. *)
-  (*       intro; simpl; reflexivity. *)
-  (*     } *)
-  (*     iRewrite "HEQ". *)
-  (*     iEval (iPureIntro; etrans). *)
-  (*     trans (reify (k2 (Vis op i k1)) σ1). *)
-  (*     simpl. *)
-  (*     (* pose proof hom_vis. *) *)
-  (*     (* rewrite H.       *) *)
-  (*     (* iRewrite - "Hs". *) *)
-  (*     (* rewrite reify_vis_eq; last first. *) *)
-  (*     (* { by rewrite Hre. } *) *)
-  (*     (* iRewrite "Hk". *) *)
-  (*     (* rewrite -Tick_eq. *) *)
-  (*     (* done. *) *)
-  (*     (* reflexivity. *) *)
-  (*     (* rewrite term *) *)
-  (*     (* iApply prod_equivI. simpl.       *) *)
-  (*     (* iSplit; eauto. *) *)
-  (*     (* iApply Tau_inj'. iRewrite "Hk". *) *)
-  (*     (* rewrite laterO_map_Next. done. *) *)
-  (* Admitted. *)
+  Lemma reify_vis_cont op i k1 k2 σ1 σ2 β
+    {PROP : bi} `{!BiInternalEq PROP} `{H : !(@CtxIndep IT _ op)} :
+    (reify (Vis op i k1) σ1 ≡ (σ2, Tick β) ⊢
+     reify (Vis op i (laterO_map k2 ◎ k1)) σ1 ≡ (σ2, Tick (k2 β)) : PROP)%I.
+  Proof.
+    destruct (sReifier_re r op (i, σ1, k1)) as [[o σ2']|] eqn:Hre; last first.
+    - rewrite (reify_vis_None _ _ k1); last by rewrite Hre//.
+      iIntros "Hr". iExFalso.
+      iPoseProof (prod_equivI with "Hr") as "[_ Hk]".
+      simpl. iApply (IT_tick_err_ne). by iApply internal_eq_sym.
+    - destruct H as [[f H]].
+      pose proof (H i σ1 k1) as H1.
+      pose proof (H i σ1 (laterO_map k2 ◎ k1)) as H2.
+      assert (∃ o σ', f (i, σ1) = Some (o, σ')) as [o' [σ' H3]].
+      {
+        destruct (f (i, σ1)) as [[? ?] | ?]; first (do 2 eexists; reflexivity).
+        simpl in H1. rewrite Hre in H1; inversion H1.
+      }
+      rewrite H3 in H1.
+      simpl in H1.
+      rewrite H3 in H2.
+      simpl in H2.
+      clear f H H3 Hre.
+      rewrite reify_vis_eq; last first.
+      { by rewrite H1. }
+      rewrite reify_vis_eq; last first.
+      { by rewrite H2. }
+      iIntros "Hr".
+      iPoseProof (prod_equivI with "Hr") as "[Hs Hk]".
+      iApply prod_equivI. simpl. iSplit; eauto.
+      iPoseProof (Tau_inj' with "Hk") as "Hk".
+      iApply Tau_inj'. iRewrite "Hk".
+      rewrite laterO_map_Next. done.
+  Qed.
 
-  (* Lemma reify_input_cont_inv op i (k1 : _ -n> laterO IT) (k2 : IT -n> IT) σ1 σ2 β *)
-  (*   {PROP : bi} `{!BiInternalEq PROP} *)
-  (*   (g : (IT -n> IT) -n> (prodO (stateF ♯ IT) IT) -n> (prodO (stateF ♯ IT) IT)) *)
-  (*   (H : reify (Vis op i (laterO_map k2 ◎ k1)) σ1 ≡ (g k2) (reify (Vis op i k1) σ1)) *)
-  (*   : *)
-  (*   (reify (Vis op i (laterO_map k2 ◎ k1)) σ1 ≡ (σ2, Tick β) *)
-  (*    ⊢ ∃ α, reify (Vis op i k1) σ1 ≡ (σ2, Tick α) ∧ ▷ (β ≡ k2 α) *)
-  (*     : PROP)%I. *)
-  (* Proof. *)
-  (*   destruct (sReifier_re r op (i, σ1, (laterO_map k2 ◎ k1))) as [[o σ2']|] eqn:Hre; last first. *)
-  (*   - rewrite reify_vis_None; last by rewrite Hre//. *)
-  (*     iIntros "Hr". iExFalso. *)
-  (*     iPoseProof (prod_equivI with "Hr") as "[_ Hk]". *)
-  (*     simpl. iApply (IT_tick_err_ne). by iApply internal_eq_sym. *)
-  (*   - rewrite reify_vis_eq; last first. *)
-  (*     { by rewrite Hre. } *)
-  (*     iIntros "Hr". simpl. *)
-  (*     iPoseProof (prod_equivI with "Hr") as "[#Hs #Hk]". *)
-  (*     simpl. *)
-  (*     iPoseProof (Tau_inj' with "Hk") as "Hk'".       *)
-  (*     destruct (Next_uninj o) as [a Hk1]. *)
-  (*     iExists (a). *)
-  (*     assert (Hre' : sReifier_re r op (i, σ1, laterO_map k2 ◎ k1) ≡ Some (o, σ2')). *)
-  (*     { by rewrite Hre. } *)
-  (*     apply reify_vis_eq in Hre'. *)
-  (*     rewrite Hre' in H. *)
-  (*     rewrite H. *)
-  (*     iRewrite - "Hr". *)
-  (*     epose proof (reify_vis_eq _ _ _ _ _ _ Hre). *)
-  (*     rewrite reify_vis_eq; last first. *)
-  (*     { by rewrite H1. } *)
-  (*     iSplit. *)
-  (*     + iApply prod_equivI. simpl. iSplit; eauto. *)
-  (*       iApply Tau_inj'. done. *)
-  (*     + iAssert (laterO_map k2 (Next a) ≡ Next β)%I as "Ha". *)
-  (*       { *)
-  (*         iSimpl in "Hk'". iRewrite -"Hk'". *)
-  (*         iPureIntro. rewrite -Hk1. *)
-  (*         rewrite Hre in H2. *)
-  (*         inversion H2 as [? ? H2' |]; subst; inversion H2'; simpl in *; subst. *)
-  (*         symmetry; assumption. *)
-  (*       } *)
-  (*       iAssert (Next (k2 a) ≡ Next β)%I as "Hb". *)
-  (*       { iRewrite -"Ha". iPureIntro. *)
-  (*         rewrite laterO_map_Next. done. } *)
-  (*       iNext. by iApply internal_eq_sym. *)
-  (* Qed. *)
+  Lemma reify_input_cont_inv op i (k1 : _ -n> laterO IT) (k2 : IT -n> IT) σ1 σ2 β
+    {PROP : bi} `{!BiInternalEq PROP} `{H : !(@CtxIndep IT _ op)} :
+    (reify (Vis op i (laterO_map k2 ◎ k1)) σ1 ≡ (σ2, Tick β)
+     ⊢ ∃ α, reify (Vis op i k1) σ1 ≡ (σ2, Tick α) ∧ ▷ (β ≡ k2 α)
+         : PROP)%I.
+  Proof.
+    destruct (sReifier_re r op (i, σ1, (laterO_map k2 ◎ k1))) as [[o σ2']|] eqn:Hre; last first.
+    - rewrite reify_vis_None; last by rewrite Hre//.
+      iIntros "Hr". iExFalso.
+      iPoseProof (prod_equivI with "Hr") as "[_ Hk]".
+      simpl. iApply (IT_tick_err_ne). by iApply internal_eq_sym.
+    - rewrite reify_vis_eq; last first.
+      { by rewrite Hre. }
+      iIntros "Hr". simpl.
+      iPoseProof (prod_equivI with "Hr") as "[#Hs #Hk]".
+      simpl.
+      iPoseProof (Tau_inj' with "Hk") as "Hk'".
+      destruct H as [[f H]].
+      pose proof (H i σ1 k1) as H1.
+      pose proof (H i σ1 (laterO_map k2 ◎ k1)) as H2.
+      assert (∃ o, f (i, σ1) ≡ Some (o, σ2')) as [o' H3].
+      {
+        destruct (f (i, σ1)) as [[? ?] | ?].
+        - simpl in H2.
+          rewrite Hre in H2.
+          inversion H2 as [? ? H2' |]; subst; inversion H2'; simpl in *; subst.
+          eexists _; do 2 f_equiv; first reflexivity; symmetry; assumption.
+        - simpl in H2.
+          rewrite Hre in H2.
+          inversion H2.
+      }
+      rewrite H3 in H1.
+      simpl in H1.
+      rewrite H3 in H2.
+      simpl in H2.
+      destruct (Next_uninj (k1 o')) as [a Hk1].
+      iExists (a).
+      rewrite reify_vis_eq; last first.
+      { by rewrite H1. }
+      iSplit.
+      + iApply prod_equivI. simpl. iSplit; eauto.
+        iApply Tau_inj'. done.
+      + iAssert (laterO_map k2 (Next a) ≡ Next β)%I as "Ha".
+        {
+          iSimpl in "Hk'". iRewrite -"Hk'".
+          iPureIntro. rewrite -Hk1.
+          rewrite Hre in H2.
+          inversion H2 as [? ? H2' |]; subst; inversion H2'; simpl in *; subst.
+          symmetry; assumption.
+        }
+        iAssert (Next (k2 a) ≡ Next β)%I as "Hb".
+        { iRewrite -"Ha". iPureIntro.
+          rewrite laterO_map_Next. done. }
+        iNext. by iApply internal_eq_sym.
+  Qed.
 
 End reifiers.
